<?xml version="1.0"?>
<rdf:RDF xmlns="http://www.semanticweb.org/kalyan/ontologies/2021/10/untitled-ontology-14#"
     xml:base="http://www.semanticweb.org/kalyan/ontologies/2021/10/untitled-ontology-14"
     xmlns:law="http://www.semanticweb.org/law#"
     xmlns:owl="http://www.w3.org/2002/07/owl#"
     xmlns:rdf="http://www.w3.org/1999/02/22-rdf-syntax-ns#"
     xmlns:xml="http://www.w3.org/XML/1998/namespace"
     xmlns:xsd="http://www.w3.org/2001/XMLSchema#"
     xmlns:rdfs="http://www.w3.org/2000/01/rdf-schema#">
    <owl:Ontology rdf:about="http://www.semanticweb.org/law"/>
    


    <!-- 
    ///////////////////////////////////////////////////////////////////////////////////////
    //
    // Annotation properties
    //
    ///////////////////////////////////////////////////////////////////////////////////////
     -->

    


    <!-- http://www.semanticweb.org/law#definekeywords -->

    <owl:AnnotationProperty rdf:about="http://www.semanticweb.org/law#definekeywords"/>
    


    <!-- 
    ///////////////////////////////////////////////////////////////////////////////////////
    //
    // Object Properties
    //
    ///////////////////////////////////////////////////////////////////////////////////////
     -->

    


    <!-- http://www.semanticweb.org/law#CombinableProperty -->

    <owl:ObjectProperty rdf:about="http://www.semanticweb.org/law#CombinableProperty">
        <rdfs:subPropertyOf rdf:resource="http://www.w3.org/2002/07/owl#topObjectProperty"/>
        <rdfs:comment rdf:datatype="http://www.w3.org/2001/XMLSchema#string">Properties whose values can be combined to a subject&apos;s instance are sub-properties of this property.</rdfs:comment>
    </owl:ObjectProperty>
    


    <!-- http://www.semanticweb.org/law#against -->

    <owl:ObjectProperty rdf:about="http://www.semanticweb.org/law#against">
        <rdfs:subPropertyOf rdf:resource="http://www.semanticweb.org/law#CombinableProperty"/>
        <rdfs:domain rdf:resource="http://www.semanticweb.org/law#case"/>
        <rdfs:range rdf:resource="http://www.semanticweb.org/law#defendant"/>
        <rdfs:comment>This property is used to know against whom the case has been filed.</rdfs:comment>
    </owl:ObjectProperty>
    


    <!-- http://www.semanticweb.org/law#filed -->

    <owl:ObjectProperty rdf:about="http://www.semanticweb.org/law#filed">
        <rdfs:subPropertyOf rdf:resource="http://www.w3.org/2002/07/owl#topObjectProperty"/>
        <rdfs:domain rdf:resource="http://www.semanticweb.org/law#plaintiff"/>
        <rdfs:range rdf:resource="http://www.semanticweb.org/law#case"/>
        <rdfs:comment>This property is used to know about the relation between plaintiff the case, and what type of case the plaintiff filed.</rdfs:comment>
    </owl:ObjectProperty>
    


    <!-- http://www.semanticweb.org/law#in -->

    <owl:ObjectProperty rdf:about="http://www.semanticweb.org/law#in">
        <rdfs:subPropertyOf rdf:resource="http://www.w3.org/2002/07/owl#topObjectProperty"/>
        <rdfs:domain rdf:resource="http://www.semanticweb.org/law#case"/>
        <rdfs:range rdf:resource="http://www.semanticweb.org/law#courtplace"/>
        <rdfs:comment>This property is used to know where the case has been filed.</rdfs:comment>
    </owl:ObjectProperty>
    


    <!-- 
    ///////////////////////////////////////////////////////////////////////////////////////
    //
    // Data properties
    //
    ///////////////////////////////////////////////////////////////////////////////////////
     -->

    


    <!-- http://www.semanticweb.org/law#KeywordProperty -->

    <owl:DatatypeProperty rdf:about="http://www.semanticweb.org/law#KeywordProperty">
        <rdfs:subPropertyOf rdf:resource="http://www.w3.org/2002/07/owl#topDataProperty"/>
        <rdfs:comment>Properties that uses keywords are sub-properites of this KeywordProperty property.</rdfs:comment>
    </owl:DatatypeProperty>
    


    <!-- http://www.semanticweb.org/law#allege -->

    <owl:DatatypeProperty rdf:about="http://www.semanticweb.org/law#allege">
        <rdfs:subPropertyOf rdf:resource="http://www.semanticweb.org/law#KeywordProperty"/>
        <rdfs:domain rdf:resource="http://www.semanticweb.org/law#plaintiff"/>
        <rdfs:range rdf:resource="http://www.w3.org/2001/XMLSchema#string"/>
        <law:definekeywords rdf:datatype="http://www.w3.org/2001/XMLSchema#string">alleging that
allege that
alleged
alleges
allegations for</law:definekeywords>
        <rdfs:comment>This property is used to get the information about the plaintiffs allegations.</rdfs:comment>
    </owl:DatatypeProperty>
    


    <!-- http://www.semanticweb.org/law#argue -->

    <owl:DatatypeProperty rdf:about="http://www.semanticweb.org/law#argue">
        <rdfs:subPropertyOf rdf:resource="http://www.semanticweb.org/law#KeywordProperty"/>
        <rdfs:domain rdf:resource="http://www.semanticweb.org/law#defendant"/>
        <rdfs:range rdf:resource="http://www.w3.org/2001/XMLSchema#string"/>
        <law:definekeywords rdf:datatype="http://www.w3.org/2001/XMLSchema#string">argues that
said that
claim that</law:definekeywords>
        <rdfs:comment>This property is used to know about the arguments from the defendents.</rdfs:comment>
    </owl:DatatypeProperty>
    


    <!-- http://www.semanticweb.org/law#decision -->

    <owl:DatatypeProperty rdf:about="http://www.semanticweb.org/law#decision">
        <rdfs:subPropertyOf rdf:resource="http://www.semanticweb.org/law#KeywordProperty"/>
        <rdfs:domain rdf:resource="http://www.semanticweb.org/law#judge"/>
        <rdfs:range rdf:resource="http://www.w3.org/2001/XMLSchema#string"/>
        <law:definekeywords rdf:datatype="http://www.w3.org/2001/XMLSchema#string">issued a default judgment
issued its decision
issued a judgment, 
issued a final verdict</law:definekeywords>
        <rdfs:comment>This property is used to know about the decision by the Judge.</rdfs:comment>
    </owl:DatatypeProperty>
    


    <!-- http://www.semanticweb.org/law#demands -->

    <owl:DatatypeProperty rdf:about="http://www.semanticweb.org/law#demands">
        <rdfs:subPropertyOf rdf:resource="http://www.semanticweb.org/law#KeywordProperty"/>
        <rdfs:domain rdf:resource="http://www.semanticweb.org/law#plaintiff"/>
        <rdfs:range rdf:resource="http://www.w3.org/2001/XMLSchema#string"/>
        <law:definekeywords rdf:datatype="http://www.w3.org/2001/XMLSchema#string">demanding
request
seek orders, 
want</law:definekeywords>
        <rdfs:comment>This property is used to know the plaintiffs demands.</rdfs:comment>
    </owl:DatatypeProperty>
    


    <!-- http://www.semanticweb.org/law#on -->

    <owl:DatatypeProperty rdf:about="http://www.semanticweb.org/law#on">
        <rdfs:subPropertyOf rdf:resource="http://www.semanticweb.org/law#KeywordProperty"/>
        <rdfs:domain rdf:resource="http://www.semanticweb.org/law#proceedings"/>
        <rdfs:range rdf:resource="http://www.w3.org/2001/XMLSchema#dateTime"/>
        <law:definekeywords rdf:datatype="http://www.w3.org/2001/XMLSchema#string">On
In</law:definekeywords>
        <rdfs:comment>This property is used to know when the proceedings had happened.</rdfs:comment>
    </owl:DatatypeProperty>
    


    <!-- 
    ///////////////////////////////////////////////////////////////////////////////////////
    //
    // Classes
    //
    ///////////////////////////////////////////////////////////////////////////////////////
     -->

    


    <!-- http://www.semanticweb.org/law#KeywordClass -->

    <owl:Class rdf:about="http://www.semanticweb.org/law#KeywordClass">
        <rdfs:comment>Classes that uses keywords are sub-class of this KeywordClass class.</rdfs:comment>
    </owl:Class>
    


    <!-- http://www.semanticweb.org/law#SummarizableClass -->

    <owl:Class rdf:about="http://www.semanticweb.org/law#SummarizableClass">
        <rdfs:comment>Classes which are primarily summarized are sub-classes of this SummarizableClass class.</rdfs:comment>
    </owl:Class>
    


    <!-- http://www.semanticweb.org/law#case -->

    <owl:Class rdf:about="http://www.semanticweb.org/law#case">
        <rdfs:subClassOf rdf:resource="http://www.semanticweb.org/law#KeywordClass"/>
        <law:definekeywords rdf:datatype="http://www.w3.org/2001/XMLSchema#string">a lawsuit
a class action
a suit
a criminal case</law:definekeywords>
        <rdfs:comment>This class is about the cases which are filed, it uses keywords.</rdfs:comment>
    </owl:Class>
    


    <!-- http://www.semanticweb.org/law#courtplace -->

    <owl:Class rdf:about="http://www.semanticweb.org/law#courtplace">
        <rdfs:subClassOf rdf:resource="http://www.semanticweb.org/law#SummarizableClass"/>
        <rdfs:comment>This class is about the places where the case has been filed.</rdfs:comment>
    </owl:Class>
    


    <!-- http://www.semanticweb.org/law#defendant -->

    <owl:Class rdf:about="http://www.semanticweb.org/law#defendant">
        <rdfs:subClassOf rdf:resource="http://www.semanticweb.org/law#SummarizableClass"/>
        <owl:disjointWith rdf:resource="http://www.semanticweb.org/law#plaintiff"/>
        <rdfs:comment>This class is about the defendents against whom the case has been filed.</rdfs:comment>
    </owl:Class>
    


    <!-- http://www.semanticweb.org/law#judge -->

    <owl:Class rdf:about="http://www.semanticweb.org/law#judge">
        <rdfs:subClassOf rdf:resource="http://www.semanticweb.org/law#KeywordClass"/>
        <law:definekeywords>the court
Judge
cheif justice</law:definekeywords>
        <rdfs:comment>This is the class about the judge and this depends on the keyords.</rdfs:comment>
    </owl:Class>
    


    <!-- http://www.semanticweb.org/law#plaintiff -->

    <owl:Class rdf:about="http://www.semanticweb.org/law#plaintiff">
        <rdfs:subClassOf rdf:resource="http://www.semanticweb.org/law#SummarizableClass"/>
        <rdfs:comment>This class is about the plaintiff&apos;s who filed the case.</rdfs:comment>
    </owl:Class>
    


    <!-- http://www.semanticweb.org/law#proceedings -->

    <owl:Class rdf:about="http://www.semanticweb.org/law#proceedings">
        <rdfs:subClassOf rdf:resource="http://www.semanticweb.org/law#KeywordClass"/>
        <law:definekeywords>legal proceedings</law:definekeywords>
        <rdfs:comment>This class is about the proceedings in the case and uses keywords from the documents to get the information.</rdfs:comment>
    </owl:Class>
    


    <!-- 
    ///////////////////////////////////////////////////////////////////////////////////////
    //
    // General axioms
    //
    ///////////////////////////////////////////////////////////////////////////////////////
     -->

    <rdf:Description>
        <rdf:type rdf:resource="http://www.w3.org/2002/07/owl#AllDisjointClasses"/>
        <owl:members rdf:parseType="Collection">
            <rdf:Description rdf:about="http://www.semanticweb.org/law#case"/>
            <rdf:Description rdf:about="http://www.semanticweb.org/law#judge"/>
            <rdf:Description rdf:about="http://www.semanticweb.org/law#proceedings"/>
        </owl:members>
    </rdf:Description>
</rdf:RDF>



<!-- Generated by the OWL API (version 4.5.9.2019-02-01T07:24:44Z) https://github.com/owlcs/owlapi -->

